\documentclass {article}
\usepackage {amsmath}
\begin {document}
Resolver los siguientes problemas sobre redes de creencias basados en el ejemplo del libro de texto:
\begin {enumerate}
	\item $P(((M \lor J) \land A) \mid (H \land \neg S))$
	\item $P (M \land \neg A \mid S)$
	\item $P ( \neg(M \lor J) \mid H)$
	\item $P ( (S \lor H) \mid (A \land J) )$
	\item $P ( \neg(M \lor J) \mid (H \lor S))$
\end {enumerate}

\clearpage
\section {Ejercicio 1}
$$P(((M \lor J) \land A) \mid (H \land \neg S))$$
$$\frac
	{P(((M \lor J) \land A) \land (H \land \neg S))}
	{P(H \land \neg S)}$$
$$\frac
	{P((M \land A \land H \land \neg S) \lor (J \land A \land H \land \neg S))}
	{P(H \land \neg S)}$$
$$\frac
	{P((M \land A \land H \land \neg S) ) + P ( (J \land A \land H \land \neg S)) - P (M \land J \land A \land H \land \neg S))}
	{P(H \land \neg S)}$$
$$\frac
	{(6.567 + 8.443 - 5.910) \cdot 10^{-4}}
	{9.98 \cdot 10^{-4}} \approx 9.12 \cdot 10^{-1}$$
\\
\\
$P((M \land A \land H \land \neg S)$\\
	\indent $
		= P(M \mid A)
		\cdot P(A \mid H \land \neg S)
		\cdot P (H)
		\cdot P(\neg S)$\\
	\indent $
		= 0.7
		\cdot 0.94
		\cdot 0.001
		\cdot 0.998 $\\
	\indent $
		\approx 6.567 \cdot 10^{-4}$
\\
\\
$P((J \land A \land H \land \neg S) $\\
	\indent $ 
		= P(J \mid A)
		\cdot P(A \mid H \land \neg S)
		\cdot P (H)
		\cdot P(\neg S)$\\
	\indent $
		= 0.9
		\cdot 0.94 
		\cdot 0.001 
		\cdot 0.998 $\\
	\indent $
		\approx 8.443 \cdot 10^{-4} $
\\
\\
$P((M \land J \land A \land H \land \neg S)$\\
	\indent $ 
		= P(J \mid A) 
		\cdot P(M \mid A) 
		\cdot P(A \mid H \land \neg S) 
		\cdot P (H) 
		\cdot P(\neg S)$\\
	\indent$ 
		= 0.9 
		\cdot 0.7 
		\cdot 0.94 
		\cdot 0.001 
		\cdot 0.998 $\\
	\indent $
		\approx 5.910 \cdot 10^{-4} $
\\
\\
$P(H \land \neg S)$\\
	\indent $ 
		= P(H) 
		\cdot P(\neg S)$\\
	\indent 
		$ = 0.01 
		\cdot 0.998 $\\
	\indent $
		= 9.98 
		\cdot 10^{-4}$

\clearpage
\section {Ejercicio 2}
$$P (M \land \neg A \mid S)$$
$$\frac
	{P (M \land \neg A \land S)}
	{P (S)}$$
$$\frac
	{1.419 \cdot 10^{-5}}
	{2 \cdot 10^{-3}} \approx 7.09 \cdot 10^{-3}$$
\\
$P(M \land \neg A \land S)$\\
	\indent $ 
		= P(M \land \neg A \land H \land S) 
		+ P(M \land \neg A \land \neg H \land S)$\\
	\indent $ 
		= 1 \cdot 10^{-9} 
		+ 1.419 \cdot 10^{-5}$\\
	\indent $ 
		\approx 1.419 \cdot 10^{-5} $\\
\\
$P(M \land \neg A \land H \land S)$\\
	\indent $ 
		= P(M \mid \neg A) 
		\cdot P(\neg A \mid H \land S) 
		\cdot P (H) 
		\cdot P (S)$\\
	\indent $ 
		= 0.01 
		\cdot 0.05 
		\cdot 0.001 
		\cdot 0.002$\\
	\indent $ =
		 1 \cdot 10^{-9}$\\
\\
$P(M \land \neg A \land \neg H \land S)$\\
	\indent $ 
		= P(M \mid \neg A) 
		\cdot P(\neg A \mid \neg H \land S) 
		\cdot P (\neg H) 
		\cdot P (S)$\\
	\indent $ 
		= 0.01 
		\cdot 0.71 
		\cdot 0.999 
		\cdot 0.002$\\
	\indent $ 
		\approx 1.419 \cdot 10^{-5}$\\


\clearpage
\section {Ejercicio 3}
$$P ( \neg(M \lor J) \mid H)$$
$$\frac
	{P (\neg M \land \neg J \land H)}
	{P(H)}$$\\
$$\frac
	{8.461 \cdot 10^{-5}}
	{1\cdot 10^{-3}}
	\approx 8.46 \cdot 10^{-2}$$\\
\\
$P (\neg M \land \neg J \land H) $\\
	\indent $ 
		= P (\neg M \land \neg J \land A \land H \land S)
		+ P (\neg M \land \neg J \land \neg A \land H \land S) 
		+ P (\neg M \land \neg J \land A \land H \land S) 
		+ P (\neg M \land \neg J \land \neg A \land H \land S)$\\
	\indent $
		\approx 5.7 \cdot 10^{-8} 
		+ 9.405 \cdot 10^{-8} 
		+ 2.814 \cdot 10^{-5} 
		+ 5.632 \cdot 10^{-5}$\\
	\indent $ 
		\approx 8.461 \cdot 10^{-5}$\\
\\
$P (\neg M \land \neg J \land A \land H \land S)$\\
	\indent $ 
		= P(\neg M \mid A) 
		\cdot P (\neg J \mid A) 
		\cdot P (A \mid H \land S) 
		\cdot P (H) 
		\cdot P (S) $\\
	\indent $ 
		= 0.3 
		\cdot 0.1 
		\cdot 0.95 
		\cdot 0.001 
		\cdot 0.002$\\
	\indent $
		\approx 5.7 \cdot 10^{-8}$\\
\\
$P (\neg M \land \neg J \land \neg A \land H \land S)$\\
	\indent $ 
		= P(\neg M \mid \neg A) 
		\cdot P (\neg J \mid \neg A) 
		\cdot P (\neg A \mid H \land S) 
		\cdot P (H) 
		\cdot P (S) $\\
	\indent $ 
		= 0.99 
		\cdot 0.95
		\cdot 0.05
		\cdot 0.001
		\cdot 0.002$\\
	\indent $ \approx 9.405 \cdot 10^{-8}$\\
\\
$P (\neg M \land \neg J \land A \land H \land \neg S)$\\
	\indent $ 
		= P(\neg M \mid A) 
		\cdot P (\neg J \mid A) 
		\cdot P (A \mid H \land \neg S) 
		\cdot P (H) 
		\cdot P (\neg S) $\\
	\indent $ 
		= 0.3 
		\cdot 0.1 
		\cdot 0.94 
		\cdot 0.001 
		\cdot 0.998$\\
	\indent $ \approx 2.814 \cdot 10^{-5} $\\
\\
$P (\neg M \land \neg J \land \neg A \land H \land \neg S)$\\
	\indent $ 
		= P(\neg M \mid \neg A) 
		\cdot P (\neg J \mid \neg A) 
		\cdot P (\neg A \mid H \land \neg S) 
		\cdot P (H) 
		\cdot P (\neg S) $\\
	\indent $ 
		= 0.99 
		\cdot 0.95
		\cdot 0.06
		\cdot 0.001 
		\cdot 0.998$\\
	\indent $ 
		\approx 5.632 \cdot 10^{-5}$\\


\clearpage
\section {Ejercicio 4}

$$P ( (S \lor H) \mid (A \land J) )$$
$$\frac
	{P ( (S \lor H) \land (A \land J) )}
	{P (A \land J)}$$
$$\frac
	{P ( (S \land A \land J) \lor (H \land A \land J) )}
	{P(A \land J)}$$
$$\frac
	{P (S \land A \land J) + P(H \land A \land J) -P(S\land H \land A \land J)}
	{P(A \land J) )}$$\\
$$\frac
	{5.232 \cdot 10^{-4} + 8.460 \cdot 10^{-4} - 1.71 \cdot 10^{-6}}
	{2.265 \cdot 10^{-3}}$$\\
$$\frac
	{1.367 \cdot 10^{-3}}
	{2.265 \cdot 10^{-3}}
	\approx 6.04 \cdot 10^{-1}$$\\
\\
$P (S \land A \land J)$\\
	\indent $ 
		= P (J \land A \land H \land S) 
		+ P (J \land A \land \neg H \land S)$\\
	\indent $ 
		\approx 1.71 \cdot 10^{-6} 
		+ 5.215 \cdot 10^{-4} $\\
	\indent $ 
		\approx 5.232 \cdot 10^{-4}$\\
\\
$P (J \land A \land H \land S)$\\
	\indent $ 
		= P(J \mid A) 
		\cdot P(A \mid H \land S) 
		\cdot P (H) 
		\cdot P (S) $\\
	\indent $ 
		= 0.9 
		\cdot 0.95 
		\cdot 0.001 
		\cdot 0.002$\\
	\indent $ 
		\approx 1.71 
		\cdot 10^{-6}$\\
\\
$P (J \land A \land \neg H \land S)$\\
	\indent $ 
		= P(J \mid A) 
		\cdot P(A \mid \neg H \land S) 
		\cdot P (\neg H) 
		\cdot P (S) $\\
	\indent $ 
		= 0.9 
		\cdot 0.29 
		\cdot 0.999 
		\cdot 0.002$\\
	\indent $ 
		\approx 5.215 \cdot 10^{-4}$\\
\\
$P (H \land A \land J)$\\
	\indent $ 
		= P (J \land A \land H \land S) 
		+ P (J \land A \land H \land \neg S)$\\
	\indent $ 
		\approx 1.71 \cdot 10^{-6} 
		+ 8.443 \cdot 10^{-4} $\\
	\indent $ 
		\approx 8.460 \cdot 10^{-4}$\\
\\
$P (A \land J)$\\
	\indent $
		= P(J \land A \land H \land S)
		+ P(J \land A \land \neg H \land S)
		+ P(J \land A \land H \land \neg S)
		+ P(J \land A \land \neg H \land \neg S)
	 $\\
 	\indent $
		= 1.71 \cdot 10^{-6}
		+ 5.215 \cdot 10^{-4}
		+ 8.443 \cdot 10^{-4}
		+ 8.973 \cdot 10^{-4}
	 $\\
	 \indent $
	 	\approx 2.265 \cdot 10^{-3}
	 $\\
\\
$P (J \land A \land \neg H \land \neg S)$\\
	\indent $
		= P (J \mid A)
		\cdot P (A \mid \neg H \land \neg S)
		\cdot P (\neg H)
		\cdot P (\neg S)$\\
	\indent $
		= 0.9
		\cdot 0.001
		\cdot 0.999
		\cdot 0.998
		$\\
	\indent $
		\approx 8.973 \cdot 10^{-4}$

\clearpage
\section {Ejercicio 5}
$$P ( \neg(M \lor J) \mid (H \lor S))$$

$$\frac
	{P (( \neg M \land \neg J) \land (H \lor S))}
	{P(H \lor S)}$$

$$\frac
	{P (( \neg M \land \neg J \land H) \lor (\neg M \land \neg J \land S))}
	{P(H \lor S)}$$

$$\frac
	{P ( \neg M \land \neg J \land H) + P (\neg M \land \neg J \land S) - P(\neg M \land \neg J \land H \land S)}
	{P (H) + P (S) -P (H \land S)}$$
\\

$$\frac
	{8.461 \cdot 10^{-5} + 1.351 \cdot 10^{-3} - 1.747 \cdot 10^{-5}}
	{1 \cdot 10^{-3} + 2 \cdot 10^{-3} - 2 \cdot 10^{-6}}$$
\\

$$\frac
	{1.418 \cdot 10^{-3}}
	{2.998 \cdot 10^{-3}}
	\approx 4.73 \cdot 10^{-1}
	$$
\\
$P(\neg M \land \neg J \land S)$\\
	\indent $
		= P(\neg M \land \neg J \land A \land S)
		+ P(\neg M \land \neg J \land \neg A \land S)
		$\\
	\indent $\approx 1.744 \cdot 10^{-5} + 1.334 \cdot 10^{-3}$\\
	\indent $\approx 1.351 \cdot 10^{-3}$\\
\\
$P(\neg M \land \neg J \land A \land S)$\\
	\indent $
		= P(\neg M \land \neg J \land A \land H \land S) 
		+ P(\neg M \land \neg J \land A \land \neg H \land S)$\\	\indent $
		= 5.7 \cdot 10^{-8}
		+ 1.738 \cdot 10^{-5}$\\
	\indent $ 1.744 \cdot 10^{-5} $\\
\\
$P(\neg M \land \neg J \land A \land \neg H \land S)$\\
	\indent $ 
		= P (\neg M \mid A)
		\cdot P (\neg J \mid A)
		\cdot P (A \mid \neg H \land S)
		\cdot P (\neg H)
		\cdot P (S)
		$\\
	\indent $
		= 0.3
		\cdot 0.1
		\cdot 0.29
		\cdot 0.999
		\cdot 0.002
	$\\
	\indent $ \approx 1.738 \cdot 10^{-5}$\\
\\
$P(\neg M \land \neg J \land \neg A \land S)$\\
	\indent $
		= P(\neg M \land \neg J \land \neg A \land H \land S) 
		+ P(\neg M \land \neg J \land \neg A \land \neg H \land S)$\\
	\indent $
		\approx 9.405 \cdot 10^{-8}
		+ 1.334 \cdot 10^{-3}
		$\\
	\indent $\approx 1.334 \cdot 10^{-3}$\\
\\
$P(\neg M \land \neg J \land \neg A \land H \land S)$\\
	\indent $
		= P(\neg M \mid \neg A)
		\cdot P(\neg J \mid \neg A)
		\cdot P(\neg A \mid H \land S)
		\cdot P(H)
		\cdot P(S)
		$\\
	\indent $
		= 0.99
		\cdot 0.95
		\cdot 0.05
		\cdot 0.001
		\cdot 0.002
		$\\
	\indent $
		\approx 9.405 \cdot 10 ^{-8}
	$
\\
$P(\neg M \land \neg J \land \neg A \land \neg H \land S)$\\
	\indent $
		= P(\neg M \mid \neg A)
		\cdot P(\neg J \mid \neg A)
		\cdot P(\neg A \mid \neg H \land S)
		\cdot P(\neg H)
		\cdot P(S)
		$\\
	\indent $
		= 0.99
		\cdot 0.95
		\cdot 0.71
		\cdot 0.999
		\cdot 0.002
	$\\
	\indent $
		\approx 1.334 \cdot 10^{-3}
	$\\
\\
$P(\neg M \land \neg J \land H \land S)$\\
	\indent $
		= P(\neg M \land \neg J \land A \land H \land S)
		+ P(\neg M \land \neg J \land \neg A\land H \land S)
		$\\
	\indent $
		\approx 1.738 \cdot 10^{-5}
		+ 9.405 \cdot 10^{-8}
		$\\
	\indent $\approx 1.747 \cdot 10^{-5}$
\end {document}